organization of what I am currently stucked

proofs/Utilities.lean
@@ -1,4 +1,5 @@
 import Lean
+import Hax
 
 open Lean Meta Elab Tactic
 
@@ -30,3 +31,45 @@ def evalRenameAutoN : Tactic := fun stx => do
         foundCount := foundCount + 1
 
     return [mvarId]
+
+--Some functions to work with how the AES matrix is represented.
+
+def zero_array : Vector u16 8 :=
+  Vector.replicate 8 (UInt16.ofBitVec <| BitVec.zero 16)
+
+def some_array : RustArray u16 8 :=
+  RustArray.ofVec (#v[
+    0b1000000000000000,
+    0b0000000000000000,
+    0b0000000000000000,
+    0b0000000000000000,
+    0b0000000000000000,
+    0b0000000000000000,
+    0b1000000000000000,
+    0b0000000000000000])
+
+-- Get an element from the bit map
+def get_elem (st : Vector u16 8) (elem_indx : Nat) (h : elem_indx < 16) : BitVec 8 :=
+  (8 : Nat).fold (init := 0) fun bt_indx _ elem =>
+    let elem_indx_fin := elem_indx
+    let elem_bt_indx := (st[bt_indx].toBitVec >>> (elem_indx_fin) &&& 1).setWidth 8
+    elem ||| (elem_bt_indx <<< bt_indx : BitVec 8)
+
+def set_elem (st : Vector u16 8) (elem_indx : Nat) (new_elem : BitVec 8) : (Vector u16 8) :=
+  (8 : Nat).fold (init := zero_array) fun bt_indx _ acc =>
+    let map_bit := st[bt_indx].toBitVec
+    let bt := BitVec.zeroExtend 16 ((new_elem >>> bt_indx) &&& 1)
+    let clear_map := (map_bit &&& ~~~((1 : BitVec 16) <<< elem_indx))
+    let new_map := clear_map ||| (bt <<< elem_indx)
+    (Vector.set acc bt_indx (UInt16.ofBitVec new_map))
+
+set_option maxRecDepth 100000
+theorem set_elem_th_3 (el : Nat) (h : el < 16) (new : BitVec 8) :
+  let vec_set := (set_elem zero_array el new)
+  get_elem vec_set el h = new := by
+  unfold get_elem set_elem zero_array
+  simp
+  match el with
+  | n + 16 => omega
+  | 0 | 1 | 2 | 3 | 4| 5 | 6 | 7 | 8 | 9 | 10 | 11 | 12 | 13 | 14 | 15 =>
+    bv_decide
