proofs/sub_bytes.lean
@@ -1,124 +1,92 @@
+
+-- Experimental lean backend for Hax
+-- The Hax prelude library can be found in hax/proof-libs/lean
 import Hax
 import Std.Tactic.Do
 import Std.Do.Triple
 import Std.Tactic.Do.Syntax
+import Std.Tactic.Do.Syntax
+import Utilities
 
-
-open Lean Meta Elab Tactic
 open Std.Do
 open Std.Tactic
-
 
 set_option mvcgen.warning false
 set_option linter.unusedVariables false
 
---Note: Given up because i am uncapable of simplifying the terms so bv_decide can
--- proceed
 
-namespace libcrux_aesgcm.platform.portable.aes_core
+namespace aes_core.sub_bytes
 
-set_option maxRecDepth 1000
-def SBOX : BitVec 2048 :=
-    0x63#8 ++ 0x7C#8 ++ 0x77#8 ++0x7B#8 ++0xF2#8 ++0x6B#8 ++0x6F#8 ++0xC5#8 ++0x30#8 ++0x01#8 ++0x67#8 ++0x2B#8 ++0xFE#8 ++0xD7#8 ++0xAB#8 ++0x76#8 ++
-    0xCA#8 ++0x82#8 ++0xC9#8 ++0x7D#8 ++0xFA#8 ++0x59#8 ++0x47#8 ++0xF0#8 ++0xAD#8 ++0xD4#8 ++0xA2#8 ++0xAF#8 ++0x9C#8 ++0xA4#8 ++0x72#8 ++0xC0#8 ++
-    0xB7#8 ++0xFD#8 ++0x93#8 ++0x26#8 ++0x36#8 ++0x3F#8 ++0xF7#8 ++0xCC#8 ++0x34#8 ++0xA5#8 ++0xE5#8 ++0xF1#8 ++0x71#8 ++0xD8#8 ++0x31#8 ++0x15#8 ++
-    0x04#8 ++0xC7#8 ++0x23#8 ++0xC3#8 ++0x18#8 ++0x96#8 ++0x05#8 ++0x9A#8 ++0x07#8 ++0x12#8 ++0x80#8 ++0xE2#8 ++0xEB#8 ++0x27#8 ++0xB2#8 ++0x75#8 ++
-    0x09#8 ++0x83#8 ++0x2C#8 ++0x1A#8 ++0x1B#8 ++0x6E#8 ++0x5A#8 ++0xA0#8 ++0x52#8 ++0x3B#8 ++0xD6#8 ++0xB3#8 ++0x29#8 ++0xE3#8 ++0x2F#8 ++0x84#8 ++
-    0x53#8 ++0xD1#8 ++0x00#8 ++0xED#8 ++0x20#8 ++0xFC#8 ++0xB1#8 ++0x5B#8 ++0x6A#8 ++0xCB#8 ++0xBE#8 ++0x39#8 ++0x4A#8 ++0x4C#8 ++0x58#8 ++0xCF#8 ++
-    0xD0#8 ++0xEF#8 ++0xAA#8 ++0xFB#8 ++0x43#8 ++0x4D#8 ++0x33#8 ++0x85#8 ++0x45#8 ++0xF9#8 ++0x02#8 ++0x7F#8 ++0x50#8 ++0x3C#8 ++0x9F#8 ++0xA8#8 ++
-    0x51#8 ++0xA3#8 ++0x40#8 ++0x8F#8 ++0x92#8 ++0x9D#8 ++0x38#8 ++0xF5#8 ++0xBC#8 ++0xB6#8 ++0xDA#8 ++0x21#8 ++0x10#8 ++0xFF#8 ++0xF3#8 ++0xD2#8 ++
-    0xCD#8 ++0x0C#8 ++0x13#8 ++0xEC#8 ++0x5F#8 ++0x97#8 ++0x44#8 ++0x17#8 ++0xC4#8 ++0xA7#8 ++0x7E#8 ++0x3D#8 ++0x64#8 ++0x5D#8 ++0x19#8 ++0x73#8 ++
-    0x60#8 ++0x81#8 ++0x4F#8 ++0xDC#8 ++0x22#8 ++0x2A#8 ++0x90#8 ++0x88#8 ++0x46#8 ++0xEE#8 ++0xB8#8 ++0x14#8 ++0xDE#8 ++0x5E#8 ++0x0B#8 ++0xDB#8 ++
-    0xE0#8 ++0x32#8 ++0x3A#8 ++0x0A#8 ++0x49#8 ++0x06#8 ++0x24#8 ++0x5C#8 ++0xC2#8 ++0xD3#8 ++0xAC#8 ++0x62#8 ++0x91#8 ++0x95#8 ++0xE4#8 ++0x79#8 ++
-    0xE7#8 ++0xC8#8 ++0x37#8 ++0x6D#8 ++0x8D#8 ++0xD5#8 ++0x4E#8 ++0xA9#8 ++0x6C#8 ++0x56#8 ++0xF4#8 ++0xEA#8 ++0x65#8 ++0x7A#8 ++0xAE#8 ++0x08#8 ++
-    0xBA#8 ++0x78#8 ++0x25#8 ++0x2E#8 ++0x1C#8 ++0xA6#8 ++0xB4#8 ++0xC6#8 ++0xE8#8 ++0xDD#8 ++0x74#8 ++0x1F#8 ++0x4B#8 ++0xBD#8 ++0x8B#8 ++0x8A#8 ++
-    0x70#8 ++0x3E#8 ++0xB5#8 ++0x66#8 ++0x48#8 ++0x03#8 ++0xF6#8 ++0x0E#8 ++0x61#8 ++0x35#8 ++0x57#8 ++0xB9#8 ++0x86#8 ++0xC1#8 ++0x1D#8 ++0x9E#8 ++
-    0xE1#8 ++0xF8#8 ++0x98#8 ++0x11#8 ++0x69#8 ++0xD9#8 ++0x8E#8 ++0x94#8 ++0x9B#8 ++0x1E#8 ++0x87#8 ++0xE9#8 ++0xCE#8 ++0x55#8 ++0x28#8 ++0xDF#8 ++
-    0x8C#8 ++0xA1#8 ++0x89#8 ++0x0D#8 ++0xBF#8 ++0xE6#8 ++0x42#8 ++0x68#8 ++0x41#8 ++0x99#8 ++0x2D#8 ++0x0F#8 ++0xB0#8 ++0x54#8 ++ 0xBB#8 ++0x16#8
+def SBOX_mat : Vector (Vector (BitVec 8) 16) 16 := #v[
+    #v[ 0x63#8, 0x7C#8, 0x77#8, 0x7B#8, 0xF2#8, 0x6B#8, 0x6F#8, 0xC5#8, 0x30#8, 0x01#8, 0x67#8, 0x2B#8, 0xFE#8, 0xD7#8, 0xAB#8, 0x76#8 ],
+    #v[ 0xCA#8, 0x82#8, 0xC9#8, 0x7D#8, 0xFA#8, 0x59#8, 0x47#8, 0xF0#8, 0xAD#8, 0xD4#8, 0xA2#8, 0xAF#8, 0x9C#8, 0xA4#8, 0x72#8, 0xC0#8 ],
+    #v[ 0xB7#8, 0xFD#8, 0x93#8, 0x26#8, 0x36#8, 0x3F#8, 0xF7#8, 0xCC#8, 0x34#8, 0xA5#8, 0xE5#8, 0xF1#8, 0x71#8, 0xD8#8, 0x31#8, 0x15#8 ],
+    #v[ 0x04#8, 0xC7#8, 0x23#8, 0xC3#8, 0x18#8, 0x96#8, 0x05#8, 0x9A#8, 0x07#8, 0x12#8, 0x80#8, 0xE2#8, 0xEB#8, 0x27#8, 0xB2#8, 0x75#8 ],
+    #v[ 0x09#8, 0x83#8, 0x2C#8, 0x1A#8, 0x1B#8, 0x6E#8, 0x5A#8, 0xA0#8, 0x52#8, 0x3B#8, 0xD6#8, 0xB3#8, 0x29#8, 0xE3#8, 0x2F#8, 0x84#8 ],
+    #v[ 0x53#8, 0xD1#8, 0x00#8, 0xED#8, 0x20#8, 0xFC#8, 0xB1#8, 0x5B#8, 0x6A#8, 0xCB#8, 0xBE#8, 0x39#8, 0x4A#8, 0x4C#8, 0x58#8, 0xCF#8 ],
+    #v[ 0xD0#8, 0xEF#8, 0xAA#8, 0xFB#8, 0x43#8, 0x4D#8, 0x33#8, 0x85#8, 0x45#8, 0xF9#8, 0x02#8, 0x7F#8, 0x50#8, 0x3C#8, 0x9F#8, 0xA8#8 ],
+    #v[ 0x51#8, 0xA3#8, 0x40#8, 0x8F#8, 0x92#8, 0x9D#8, 0x38#8, 0xF5#8, 0xBC#8, 0xB6#8, 0xDA#8, 0x21#8, 0x10#8, 0xFF#8, 0xF3#8, 0xD2#8 ],
+    #v[ 0xCD#8, 0x0C#8, 0x13#8, 0xEC#8, 0x5F#8, 0x97#8, 0x44#8, 0x17#8, 0xC4#8, 0xA7#8, 0x7E#8, 0x3D#8, 0x64#8, 0x5D#8, 0x19#8, 0x73#8 ],
+    #v[ 0x60#8, 0x81#8, 0x4F#8, 0xDC#8, 0x22#8, 0x2A#8, 0x90#8, 0x88#8, 0x46#8, 0xEE#8, 0xB8#8, 0x14#8, 0xDE#8, 0x5E#8, 0x0B#8, 0xDB#8 ],
+    #v[ 0xE0#8, 0x32#8, 0x3A#8, 0x0A#8, 0x49#8, 0x06#8, 0x24#8, 0x5C#8, 0xC2#8, 0xD3#8, 0xAC#8, 0x62#8, 0x91#8, 0x95#8, 0xE4#8, 0x79#8 ],
+    #v[ 0xE7#8, 0xC8#8, 0x37#8, 0x6D#8, 0x8D#8, 0xD5#8, 0x4E#8, 0xA9#8, 0x6C#8, 0x56#8, 0xF4#8, 0xEA#8, 0x65#8, 0x7A#8, 0xAE#8, 0x08#8 ],
+    #v[ 0xBA#8, 0x78#8, 0x25#8, 0x2E#8, 0x1C#8, 0xA6#8, 0xB4#8, 0xC6#8, 0xE8#8, 0xDD#8, 0x74#8, 0x1F#8, 0x4B#8, 0xBD#8, 0x8B#8, 0x8A#8 ],
+    #v[ 0x70#8, 0x3E#8, 0xB5#8, 0x66#8, 0x48#8, 0x03#8, 0xF6#8, 0x0E#8, 0x61#8, 0x35#8, 0x57#8, 0xB9#8, 0x86#8, 0xC1#8, 0x1D#8, 0x9E#8 ],
+    #v[ 0xE1#8, 0xF8#8, 0x98#8, 0x11#8, 0x69#8, 0xD9#8, 0x8E#8, 0x94#8, 0x9B#8, 0x1E#8, 0x87#8, 0xE9#8, 0xCE#8, 0x55#8, 0x28#8, 0xDF#8 ],
+    #v[ 0x8C#8, 0xA1#8, 0x89#8, 0x0D#8, 0xBF#8, 0xE6#8, 0x42#8, 0x68#8, 0x41#8, 0x99#8, 0x2D#8, 0x0F#8, 0xB0#8, 0x54#8, 0xBB#8, 0x16#8 ] ]
 
+  def SBOX : BitVec 2048 :=
+    0x63#8 ++ 0x7C#8 ++ 0x77#8 ++ 0x7B#8 ++ 0xF2#8 ++ 0x6B#8 ++ 0x6F#8 ++ 0xC5#8 ++ 0x30#8 ++ 0x01#8 ++ 0x67#8 ++ 0x2B#8 ++ 0xFE#8 ++ 0xD7#8 ++ 0xAB#8 ++ 0x76#8 ++
+    0xCA#8 ++ 0x82#8 ++ 0xC9#8 ++ 0x7D#8 ++ 0xFA#8 ++ 0x59#8 ++ 0x47#8 ++ 0xF0#8 ++ 0xAD#8 ++ 0xD4#8 ++ 0xA2#8 ++ 0xAF#8 ++ 0x9C#8 ++ 0xA4#8 ++ 0x72#8 ++ 0xC0#8 ++
+    0xB7#8 ++ 0xFD#8 ++ 0x93#8 ++ 0x26#8 ++ 0x36#8 ++ 0x3F#8 ++ 0xF7#8 ++ 0xCC#8 ++ 0x34#8 ++ 0xA5#8 ++ 0xE5#8 ++ 0xF1#8 ++ 0x71#8 ++ 0xD8#8 ++ 0x31#8 ++ 0x15#8 ++
+    0x04#8 ++ 0xC7#8 ++ 0x23#8 ++ 0xC3#8 ++ 0x18#8 ++ 0x96#8 ++ 0x05#8 ++ 0x9A#8 ++ 0x07#8 ++ 0x12#8 ++ 0x80#8 ++ 0xE2#8 ++ 0xEB#8 ++ 0x27#8 ++ 0xB2#8 ++ 0x75#8 ++
+    0x09#8 ++ 0x83#8 ++ 0x2C#8 ++ 0x1A#8 ++ 0x1B#8 ++ 0x6E#8 ++ 0x5A#8 ++ 0xA0#8 ++ 0x52#8 ++ 0x3B#8 ++ 0xD6#8 ++ 0xB3#8 ++ 0x29#8 ++ 0xE3#8 ++ 0x2F#8 ++ 0x84#8 ++
+    0x53#8 ++ 0xD1#8 ++ 0x00#8 ++ 0xED#8 ++ 0x20#8 ++ 0xFC#8 ++ 0xB1#8 ++ 0x5B#8 ++ 0x6A#8 ++ 0xCB#8 ++ 0xBE#8 ++ 0x39#8 ++ 0x4A#8 ++ 0x4C#8 ++ 0x58#8 ++ 0xCF#8 ++
+    0xD0#8 ++ 0xEF#8 ++ 0xAA#8 ++ 0xFB#8 ++ 0x43#8 ++ 0x4D#8 ++ 0x33#8 ++ 0x85#8 ++ 0x45#8 ++ 0xF9#8 ++ 0x02#8 ++ 0x7F#8 ++ 0x50#8 ++ 0x3C#8 ++ 0x9F#8 ++ 0xA8#8 ++
+    0x51#8 ++ 0xA3#8 ++ 0x40#8 ++ 0x8F#8 ++ 0x92#8 ++ 0x9D#8 ++ 0x38#8 ++ 0xF5#8 ++ 0xBC#8 ++ 0xB6#8 ++ 0xDA#8 ++ 0x21#8 ++ 0x10#8 ++ 0xFF#8 ++ 0xF3#8 ++ 0xD2#8 ++
+    0xCD#8 ++ 0x0C#8 ++ 0x13#8 ++ 0xEC#8 ++ 0x5F#8 ++ 0x97#8 ++ 0x44#8 ++ 0x17#8 ++ 0xC4#8 ++ 0xA7#8 ++ 0x7E#8 ++ 0x3D#8 ++ 0x64#8 ++ 0x5D#8 ++ 0x19#8 ++ 0x73#8 ++
+    0x60#8 ++ 0x81#8 ++ 0x4F#8 ++ 0xDC#8 ++ 0x22#8 ++ 0x2A#8 ++ 0x90#8 ++ 0x88#8 ++ 0x46#8 ++ 0xEE#8 ++ 0xB8#8 ++ 0x14#8 ++ 0xDE#8 ++ 0x5E#8 ++ 0x0B#8 ++ 0xDB#8 ++
+    0xE0#8 ++ 0x32#8 ++ 0x3A#8 ++ 0x0A#8 ++ 0x49#8 ++ 0x06#8 ++ 0x24#8 ++ 0x5C#8 ++ 0xC2#8 ++ 0xD3#8 ++ 0xAC#8 ++ 0x62#8 ++ 0x91#8 ++ 0x95#8 ++ 0xE4#8 ++ 0x79#8 ++
+    0xE7#8 ++ 0xC8#8 ++ 0x37#8 ++ 0x6D#8 ++ 0x8D#8 ++ 0xD5#8 ++ 0x4E#8 ++ 0xA9#8 ++ 0x6C#8 ++ 0x56#8 ++ 0xF4#8 ++ 0xEA#8 ++ 0x65#8 ++ 0x7A#8 ++ 0xAE#8 ++ 0x08#8 ++
+    0xBA#8 ++ 0x78#8 ++ 0x25#8 ++ 0x2E#8 ++ 0x1C#8 ++ 0xA6#8 ++ 0xB4#8 ++ 0xC6#8 ++ 0xE8#8 ++ 0xDD#8 ++ 0x74#8 ++ 0x1F#8 ++ 0x4B#8 ++ 0xBD#8 ++ 0x8B#8 ++ 0x8A#8 ++
+    0x70#8 ++ 0x3E#8 ++ 0xB5#8 ++ 0x66#8 ++ 0x48#8 ++ 0x03#8 ++ 0xF6#8 ++ 0x0E#8 ++ 0x61#8 ++ 0x35#8 ++ 0x57#8 ++ 0xB9#8 ++ 0x86#8 ++ 0xC1#8 ++ 0x1D#8 ++ 0x9E#8 ++
+    0xE1#8 ++ 0xF8#8 ++ 0x98#8 ++ 0x11#8 ++ 0x69#8 ++ 0xD9#8 ++ 0x8E#8 ++ 0x94#8 ++ 0x9B#8 ++ 0x1E#8 ++ 0x87#8 ++ 0xE9#8 ++ 0xCE#8 ++ 0x55#8 ++ 0x28#8 ++ 0xDF#8 ++
+    0x8C#8 ++ 0xA1#8 ++ 0x89#8 ++ 0x0D#8 ++ 0xBF#8 ++ 0xE6#8 ++ 0x42#8 ++ 0x68#8 ++ 0x41#8 ++ 0x99#8 ++ 0x2D#8 ++ 0x0F#8 ++ 0xB0#8 ++ 0x54#8 ++ 0xBB#8 ++ 0x16#8
 
+def get_elem_SBOX (row col : Nat) : BitVec 8:=
+  (SBOX >>> (((15 - row) * 16 + (15 - col)) * 8)).setWidth 8
+
+set_option maxHeartbeats 1000000
 set_option maxRecDepth 100000
-#eval (SBOX >>> 8).extractLsb 7 0
+theorem get_elem_correct (row col : Nat) (h1 : row < 16) (h2 : col < 16):
+  get_elem_SBOX row col = SBOX_mat[row][col] := by
+  unfold get_elem_SBOX SBOX SBOX_mat
+  match row with
+  | n + 16 => omega
+  | 0 | 1 | 2 | 3 | 4 | 5 | 6 | 7 | 8 | 9 | 10 | 11 | 12 | 13 | 14 | 15  =>
+    match col with
+    | n + 16 => omega
+    | 0 | 1 | 2 | 3 | 4 | 5 | 6 | 7 | 8 | 9 | 10 | 11 | 12 | 13 | 14 | 15  => rfl
 
-def SBOX_bt := SBOX
+def sub_bytes_state_spec (st : Vector u16 8) : Vector u16 8 :=
+  (16 : Nat).fold (init := zero_array) fun elem_indx h res =>
+    let elem := get_elem st elem_indx h
+    let row := (BitVec.extractLsb 7 4 elem).toFin
+    let col := (BitVec.extractLsb 3 0 elem).toFin
+    let new_elem := get_elem_SBOX row col
+    set_elem res elem_indx new_elem
 
-#eval BitVec.extractLsb 3 0 (0xFF#8)
-
-def get_SBOX (elem_indx : BitVec 8) := ((SBOX_bt >>> (elem_indx * 8)).extractLsb 7 0)
-
-def zero_array : Vector u16 8 :=
-  Vector.replicate 8 (UInt16.ofBitVec <| BitVec.zero 16)
-
-def get_elem_bitvec (st : (RustArray u16 8)) (elem_indx : Nat) (h : elem_indx < 16) : BitVec 8 :=
-  let (_, res) :=
-    BitVec.iunfoldr
-    (f := fun bt_indx acc =>
-      let st_vec := st.toVec
-      let elem_indx_fin : Fin 16 :=  ⟨elem_indx, h⟩
-      let new_bt := st_vec[bt_indx].toBitVec.getLsb (elem_indx_fin)
-      (acc, new_bt))
-    (s := 0)
-    (w := 8)
-  res
-
-
--- Get an element from the bit map
-def get_elem (st : (RustArray u16 8)) (elem_indx : Nat) (h : elem_indx < 16) : BitVec 8 :=
-  (8 : Nat).fold (init := 0) fun bt_indx _ elem =>
-    let elem_indx_fin := elem_indx
-    let elem_bt_indx := ((st.toVec)[bt_indx].toBitVec >>> (elem_indx_fin) &&& 1).setWidth 8
-    elem ||| (elem_bt_indx <<< bt_indx : BitVec 8)
-
-def some_array : RustArray u16 8 :=
-  RustArray.ofVec (#v[
-    0b1000000000000000,
-    0b0000000000000000,
-    0b0000000000000000,
-    0b0000000000000000,
-    0b0000000000000000,
-    0b0000000000000000,
-    0b0000000000000000,
-    0b0000000000000000])
-
-#check  (0b0110000000000001 : BitVec 8)
-
-#eval get_elem some_array 0 (by omega)
-
-def set_elem (st : Vector u16 8) (elem_indx : Nat) (new_elem : BitVec 8) : (Vector u16 8) :=
-  (8 : Nat).fold (init := zero_array) fun bt_indx _ acc =>
-    let map_bit := st[bt_indx].toBitVec
-    let bt := BitVec.zeroExtend 16 ((new_elem >>> bt_indx) &&& 1)
-    let new_map := map_bit ||| (bt <<< elem_indx)
-    (Vector.set acc bt_indx (UInt16.ofBitVec new_map))
-
-def sub_bytes_state_spec (st : (RustArray u16 8)) : RustArray u16 8 :=
-  RustArray.ofVec
-    (
-      (16 : Nat).fold (init := zero_array) fun elem_indx h res =>
-        let elem := get_elem_bitvec st elem_indx h
-        let row := (BitVec.extractLsb 7 4 elem)
-        let col := (BitVec.extractLsb 3 0 elem)
-        let new_elem := get_SBOX (row.setWidth 8 * 16 + col.setWidth 8)
-        set_elem res elem_indx new_elem
-    ).reverse
-
-theorem set_get_1 (input : RustArray u16 8) (new_elem : BitVec 8):
-  get_elem_bitvec input 0 (by grind) = get_elem (RustArray.ofVec (set_elem input.toVec 1 new_elem)) 0 (by grind) := by
-  unfold get_elem set_elem get_elem_bitvec
-  --simp
-  --rw [BitVec.iunfoldr_replace]
-  --exact id
-  --rfl
-  --intro i
-  --bv_decide
-  --match i with
-  --| 0 => grind
-  --| _ => sorry
-  sorry
-  --bv_decide
-
-
-
+theorem sbox_th (st : Vector u16 8) (el : BitVec 4) (h : el < 16):
+  let ⟨el_val, el_h⟩ := el
+  let elem := get_elem st el_val el_h
+  let row := (BitVec.extractLsb 7 4 elem).toFin
+  let col := (BitVec.extractLsb 3 0 elem).toFin
+  let new_elem := get_elem_SBOX row col
+  get_elem (set_elem zero_array el_val new_elem) el_val el_h = 0x22#8 :=
+by
+  unfold get_elem set_elem zero_array get_elem_SBOX SBOX
+  simp
+  bv_decide
 
 @[spec]
 def xnor (a : u16) (b : u16) : RustM u16 := do (~? (← (a ^^^? b)))
@@ -300,183 +268,53 @@ def sub_bytes_state (st : (RustArray u16 8)) : RustM (RustArray u16 8) := do
       (7 : usize)
       s0);
   (pure st)
-def aux_fun (input : RustArray u16 8) :=
-  match (sub_bytes_state input) with
-      | RustM.ok v => v
-      | _ => RustArray.ofVec zero_array
 
 
-#eval aux_fun some_array --= #[65412, 65535, 123, 0, 123, 65412, 65412, 0]
-#eval sub_bytes_state_spec some_array --= #[65412, 65412, 123, 123, 123, 65535, 65535, 0]
-
-
-/--
-Generates a name based on an index (0 -> a, 1 -> b, etc.)
--/
-def getAutoName (i : Nat) : Name :=
-    s!"var_{i}" |>.toName
-
-syntax (name := renameAutoN) "rename_auto_n " num : tactic
-
-@[tactic renameAutoN]
-def evalRenameAutoN : Tactic := fun stx => do
-  -- Parse the number 'n' from the tactic call
-  let n := stx[1].isNatLit?.getD 0
-
-  liftMetaTactic fun mvarId => do
-    let lctx ← getLCtx
-    let mut mvarId := mvarId
-    let mut foundCount := 0
-
-    for ldecl in lctx do
-      if foundCount >= n then break
-
-      -- Check if the hypothesis is inaccessible (has macro scopes or is a dagger/internal name)
-      if ldecl.userName.hasMacroScopes || ldecl.userName.toString.startsWith "✝" then
-        let newName := getAutoName foundCount
-        mvarId ← mvarId.rename ldecl.fvarId newName
-        foundCount := foundCount + 1
-
-    return [mvarId]
-
---set_option maxRecDepth 1000000
---theorem example_lemma :
---(sub_bytes_state_spec zero_array).toVec[0].toBitVec.getLsb 0 = (true : Bool) :=
---by
---  simp only [sub_bytes_state_spec]
---  simp only [set_elem, get_SBOX]
---  simp only [SBOX_bt, get_elem, SBOX]
---  simp only [zero_array]
---  simp
---  rfl
---
---def test_array : RustArray u16 8 :=
---  RustArray.ofVec (#v[
---    65535,
---    65535,
---    65535,
---    65535,
---    65535,
---    65535,
---    65535,
---    65535])
---
-
---set_option maxHeartbeats 1000000
---def example_debug (st : (RustArray u16 8)) (var_1 : BitVec 1) :
---:= by
---    bv_decide
-
-set_option maxRecDepth 1000000
-set_option maxHeartbeats 10000000
-theorem example_a (st : (RustArray u16 8)):
+set_option maxHeartbeats 1000000000
+theorem sub_bytes_correct_some_array :
 ⦃ ⌜ true = true ⌝ ⦄
-sub_bytes_state st
+sub_bytes_state some_array
 ⦃ ⇓ ⟨res_output⟩ =>
-    ⌜ (sub_bytes_state_spec st).toVec[0] = (res_output[0] : u16) ⌝ ⦄
+    ⌜ (sub_bytes_state_spec some_array.toVec) = res_output ⌝ ⦄
+:= by
+
+  unfold sub_bytes_state
+  hax_mvcgen <;> simp at *
+  .
+    ext i
+    match i with
+    | n + 16 => omega
+    | 0 | 1 | 2 | 3 | 4 | 5 | 6 | 7 | 8 | 9 | 10 | 11 | 12 | 13 | 14 | 15 =>
+      unfold sub_bytes_state_spec
+      simp only [zero_array, get_elem_SBOX, get_elem, SBOX, set_elem]
+      rename_auto_n 45
+      simp only [var_1, var_3, var_5, var_7, var_9, var_11, var_13, var_24]
+      simp
+      unfold some_array
+      simp
+      bv_normalize
+  all_goals grind
+
+set_option maxHeartbeats 1000000000
+theorem sub_bytes_correct (st : Vector u16 8):
+⦃ ⌜ true = true ⌝ ⦄
+sub_bytes_state (RustArray.ofVec st)
+⦃ ⇓ ⟨res_output⟩ =>
+    ⌜ (sub_bytes_state_spec st)[0] = res_output[0] ⌝ ⦄
 := by
     unfold sub_bytes_state
     hax_mvcgen <;> simp at *
     .
-
-      simp only [Vector.getElem_set]
-      simp only [↓reduceIte]
-      simp only [sub_bytes_state_spec]
-      simp only [set_elem, get_SBOX]
-      rename_auto_n 25
-      clear var_22 var_21 var_20 var_19 var_18 var_17 var_16 var_15
+      unfold sub_bytes_state_spec
+      simp only [zero_array, get_elem_SBOX, get_elem, SBOX, set_elem]
+      rename_auto_n 45
+      simp only [var_1, var_3, var_5, var_7, var_9, var_11, var_13, var_24]
       simp
-      simp only [SBOX_bt, get_elem_bitvec, SBOX]
-      simp
-      simp only [zero_array]
-
-
-
-      --simp only [<- var_24, <- var_13, <- var_11, <- var_9, <- var_7, <- var_5, <- var_3, <- var_1, <-var_23]
-      --bv_decide
       sorry
-    --  simp
-    --  simp only [zero_array] at *
-    --  simp at *
-    --  by_cases h1 : st.toVec[0].toBitVec[0]
-    --  sorry
-
-      --bv_decide
-    --  match st.toVec[0].toBitVec[0] with
-    --  | true =>
-    --  | false => sorry
-    --  --simp only [<- var_24, <- var_13, <- var_11, <- var_9, <- var_7, <- var_5, <- var_3, <- var_1, <-var_23]
-    --  --bv_decide
-    --clear var_24 var_13 var_11 var_9 var_7 var_5  var_3 var_1 var_23
-    --cases BitVec.extractLsb' 14 1 var_12.toBitVec == 1#1 startsWith
-
-      --bv_decide
-    --all_goals grind
-    sorry
-    --
-    --  --rw [<- var_24, <- var_13, <- var_11, <- var_9, <- var_7, <- var_5, <- var_3, <- var_1]
-
-      --simp only [<- var_24]
-      --simp only [SBOX_bt]
-      --unfold SBOX
-
       --bv_decide
 
-      --bv_decide
-      --bv_decide
-
-set_option maxHeartbeats 1000000000
-set_option pp.maxSteps 10000
-set_option hax_mvcgen.specset "bv" in
-theorem sub_bytes_correct (st : (RustArray u16 8)) (output : (RustArray u16 8)) :
-⦃ ⌜ true = true ⌝ ⦄
-sub_bytes_state st
-⦃ ⇓ ⟨res_output⟩ =>
-    ⌜ get_elem (RustArray.ofVec res_output) 0 (by omega) = get_elem (sub_bytes_state_spec st) 0 (by omega) ⌝ ⦄
-:= by
-      unfold sub_bytes_state
-      hax_mvcgen <;> simp at *
-      .
-
-        simp only [Vector.getElem_set]
-        simp only [↓reduceIte]
-        simp only [sub_bytes_state_spec]
-        simp
-        simp only [set_elem, get_SBOX]
-      --  rename_auto_n 25
-      --  clear var_22 var_21 var_20 var_19 var_18 var_17 var_16 var_15
-      -- --simp
-      --  simp only [SBOX_bt, get_elem, SBOX]
-      --  simp
-      --  simp at *
-
-      --clear var_24 var_13 var_11 var_9 var_7 var_5  var_3 var_1 var_23
-
-      --bv_decide
-    sorry
+    all_goals grind
 
 
 
-
-    --unfold sub_bytes_state
-    --hax_mvcgen
-    --<;> simp at *
-    --.
---
-    --  rename _ = st.toVec[7] => h7
-    --  rename _ = st.toVec[6] => h6
-    --  rename _ = st.toVec[5] => h5
-    --  rename _ = st.toVec[4] => h4
-    --  rename _ = st.toVec[3] => h3
-    --  rename _ = st.toVec[2] => h2
-    --  rename _ = st.toVec[1] => h1
-    --  rename _ = st.toVec[0] => h0
---
-    --  unfold sub_bytes_state_spec
-    --  simp only [Nat.fold_succ, Nat.fold_zero]
-      --simp?
-
-
-
-
-end libcrux_aesgcm.platform.portable.aes_core
+end aes_core.sub_bytes
